\documentclass{article}
\title{Problem set 1}
\usepackage{amssymb}
\usepackage{amsmath}
\author{Jose Ramirez}
\setlength{\parindent}{0pt}
\pdfpagewidth 8.5in
\pdfpageheight 11in

\begin{document}
\maketitle

So, we have our cost function:
$$
	J(\theta) = \frac{1}{m}\sum_{i = 1}^m \log(1 + e^{-y^{(i)}\theta^{T}x^{(i)}}).
$$

Let's try to find the Hessian matrix for this function. We have the following:
\begin{eqnarray*}
	\frac{\partial^2 J}{\partial{\theta_k} \partial{\theta_l}} =
	\frac{\partial}{\partial{\theta_k}}\left(\frac{\partial J}{\partial{\theta_l}}\right) =
	\frac{\partial}{\partial{\theta_k}}\left(\frac{1}{m}\sum_{i = 1}^m -h_{\theta}(-y^{(i)}x^{(i)})y^{(i)}x^{(i)}_l \right) = \\
	\frac{1}{m}\sum_{i = 1}^m h_{\theta}(y^{(i)}x^{(i)})(1 - h_{\theta}(y^{(i)}x^{(i)}))x^{(i)}_{k}x^{(i)}_{l} = \\
	\frac{1}{m}\sum_{i = 1}^m h'_{\theta}(y^{(i)}x^{(i)})x^{(i)}_{k}x^{(i)}_{l}, \\
\end{eqnarray*}

and with that, we get that:
$$
	H = \nabla^{2} J(\theta) = \frac{1}{m}\sum_{i} h'_{\theta}(y^{(i)}x^{(i)})x^{(i)}(x^{(i)})^{T}.
$$

Now to prove the inequality, we see that
$$
	z^THz = \frac{1}{m}\sum_{i = 1}^m h'_{\theta}(y^{(i)}x^{(i)})z^Tx^{(i)}(x^{(i)})^{T}z =
	\frac{1}{m}\sum_{i = 1}^m h'_{\theta}(y^{(i)}x^{(i)})(z^Tx^{(i)})^2 \geq 0,
$$
as needed.

Here we used the following results:
\begin{enumerate}
\item $$\frac{\partial}{\partial \theta_k}\log(1 + e^{-y\theta^Tx}) = -h_{\theta}(-yx)yx_k$$
\item $$\frac{\partial}{\partial \theta_i}\frac{-yx_k}{1 + e^{y\theta^Tx}} = h'_{\theta}(yx)y^2x_ix_k$$
\item $$z^Tx = x^Tz$$
\end{enumerate}
\end{document}